Primitive_Matchers/Common_Primitive_Syntax.thy
@@ -16,6 +16,7 @@ datatype common_primitive =
   is_Prot: Prot (prot_sel: protocol) | 
   is_Src_Ports: Src_Ports (src_ports_sel: ipt_ports) |
   is_Dst_Ports: Dst_Ports (dst_ports_sel: ipt_ports) |
+  is_L4_Flags: L4_Flags (l4_flags_sel: ipt_tcp_flags) |
   is_CT_State: CT_State (ct_state_sel: "ctstate set") |
   is_Extra: Extra (extra_sel: string)
 
@@ -29,6 +30,7 @@ lemma wf_disc_sel_common_primitive:
       "wf_disc_sel (is_Iiface, iiface_sel) IIface"
       "wf_disc_sel (is_Oiface, oiface_sel) OIface"
       "wf_disc_sel (is_Prot, prot_sel) Prot"
+      "wf_disc_sel (is_L4_Flags, l4_flags_sel) L4_Flags"
       "wf_disc_sel (is_CT_State, ct_state_sel) CT_State"
       "wf_disc_sel (is_Extra, extra_sel) Extra"
   by(simp_all add: wf_disc_sel.simps)
@@ -36,7 +38,7 @@ lemma wf_disc_sel_common_primitive:
 
   --"Example"
   value "\<lparr>p_iiface = ''eth0'', p_oiface = ''eth1'', p_src = ipv4addr_of_dotdecimal (192,168,2,45), p_dst= ipv4addr_of_dotdecimal (173,194,112,111),
-         p_proto=TCP, p_sport=2065, p_dport=80, p_tag_ctstate = CT_New\<rparr>"
+         p_proto=TCP, p_sport=2065, p_dport=80, p_tcp_flags = {}, p_tag_ctstate = CT_New\<rparr>"
 
 
 
