Primitive_Matchers/Simple_Packet.thy
@@ -11,7 +11,8 @@ section{*Simple Packet*}
                          p_proto :: primitive_protocol
                          p_sport :: "16 word"
                          p_dport :: "16 word"
+                         p_tcp_flags :: "tcp_flag set"
                          p_tag_ctstate :: ctstate
 
-  value "\<lparr>p_iiface = ''eth1'', p_oiface = '''', p_src = 0, p_dst = 0, p_proto = TCP, p_sport = 0, p_dport = 0, p_tag_ctstate = CT_New\<rparr>"
+  value "\<lparr>p_iiface = ''eth1'', p_oiface = '''', p_src = 0, p_dst = 0, p_proto = TCP, p_sport = 0, p_dport = 0, p_tcp_flags = {TCP_SYN}, p_tag_ctstate = CT_New\<rparr>"
 end
